(Realistično gledano nevem zakaj se oboje učimo če pr negitvnemu sam negativno število namesto pozitivnega vstaviš)$\color{blue}\;^{**}$
***
$$(a + b)^{2} = a^{2} + 2ab + b^2$$
$$(a - b)^{2} = a^{2} - 2ab + b^2\color{blue}\;^{**}$$
***
$$(a + b)^{3} = a^{3}  + b^{3} + 3a^2b + 3ab^2$$
$$(a - b)^{3} = a^{3}  - b^{3} - 3a^2b + 3ab^{2}\color{blue}\;^{**}$$
***
$$(a + b + c)^{2} = a^{2} + b^{2}+ c^{2} + 2(ac + bc + ac)$$
***
$$a^{2}- b^{2}= (a-b)(a+b)$$
$$a^{2}+ b^{2}= (a-bi)(a+bi)$$
***
$$a^{3}+ b^{3}= (a+b)(a^2-ab+b^2)$$
$$a^{3}- b^{3}= (a-b)(a^2+ab+b^2)\color{blue}\;^{**}$$
***
### Vietovo Pravilo
$$a^{2}+ (a+b)x + ab = (x+a)(x+b)$$

